push_cons

pulse/examples/steel/LListWithTail.fst
@@ -1,5 +1,6 @@
 module LListWithTail
 open Steel.Memory
+open Steel.Effect.Atomic
 open Steel.Effect
 open Steel.FractionalPermission
 open Steel.Reference
@@ -8,21 +9,203 @@ module L = FStar.List.Tot.Base
 
 noeq
 type t (a: Type0) = {
-  list: LL.t a;
+  head: ref (LL.cell a);
   tail: ref (LL.cell a);
 }
 
-let llist_with_tail (#a: Type0) (x: t a) (l: list (LL.cell a)) : Tot slprop =
-  LL.llist x.list l `star`
-  pure (is_null x.tail == Nil? l) `star`
-  begin match l with
-  | [] -> emp
-  | _ -> pts_to x.tail full_perm (L.last l)
+let null_llist (#a:Type) : Tot (t a) = {
+  head = null;
+  tail = null;
+}
+
+let rec llist_with_tail_fragment (#a: Type0) (x: t a) (hd: Ghost.erased (LL.cell a)) (tl: Ghost.erased (list (LL.cell a))) : Tot slprop (decreases (Ghost.reveal tl)) =
+  pts_to x.head full_perm hd `star`
+  begin match Ghost.reveal tl with
+  | [] -> pure (x.tail == x.head)
+  | a' :: q -> llist_with_tail_fragment ({ head = LL.next hd; tail = x.tail }) a' q
   end
 
-let empty (a: Type0) : Tot (t a) =
-  {
-    list = LL.null_llist;
-    tail = null;
-  }
+let llist_with_tail_fragment_cons
+  (#a: Type0) (x: t a) (hd: Ghost.erased (LL.cell a)) (tl: Ghost.erased (list (LL.cell a)))
+: Lemma
+  (requires (Cons? tl))
+  (ensures (llist_with_tail_fragment x hd tl == (pts_to x.head full_perm hd `star` llist_with_tail_fragment ({ head = LL.next hd; tail = x.tail }) (L.hd tl) (L.tl tl))))
+=
+  ()
+
+let llist_with_tail (#a: Type0) (x: t a) (l: Ghost.erased (list (LL.cell a))) : Tot slprop =
+  match Ghost.reveal l with
+  | [] -> pure (is_null x.head == true) `star` pure (is_null x.tail == true)
+  | hd :: tl -> llist_with_tail_fragment x hd tl `star` pure (is_null (LL.next (L.last l)) == true)
+
+let llist_with_tail_cons
+  (#a: Type0) (x: t a) (l: Ghost.erased (list (LL.cell a)))
+: Lemma
+  (requires (Cons? l))
+  (ensures (llist_with_tail x l == llist_with_tail_fragment x (L.hd l) (L.tl l) `star` pure (is_null (LL.next (L.last l)) == true)))
+= ()
+
+val pure_star_interp (p:slprop u#a) (q:prop) (m:mem)
+   : Lemma (interp (p `star` pure q) m <==>
+            interp p m /\ q)
+
+let pure_star_interp p q m =
+  pure_star_interp p q m;
+  emp_unit p
+
+val intro_llist_nil (a:Type)
+   : SteelT unit emp (fun _ -> llist_with_tail (null_llist #a) [])
+
+let intro_llist_nil a =
+  change_slprop emp (llist_with_tail (null_llist #a) [])
+    (fun m ->
+      pure_interp (is_null (null_llist #a).head == true) m;
+      pure_star_interp (pure (is_null (null_llist #a).head == true)) (is_null (null_llist #a).tail == true) m;
+      norm_spec [delta; zeta] ((llist_with_tail (null_llist #a) [])))
+
+val intro_llist_cons_nil'
+  (a: Type)
+  (ptr: t a)
+  (x: LL.cell a)
+  (m: mem)
+: Lemma
+  (requires (
+    interp (pts_to ptr.head full_perm x `star` pure (is_null (LL.next x) == true) `star` pure (ptr.tail == ptr.head)) m
+  ))
+  (ensures (interp (llist_with_tail ptr [x]) m))
+
+let intro_llist_cons_nil'
+  a ptr x m
+=
+  pure_star_interp (pts_to ptr.head full_perm x `star` pure (is_null (LL.next x) == true)) (ptr.tail == ptr.head) m;
+  pure_star_interp (pts_to ptr.head full_perm x) (is_null (LL.next x) == true) m;
+  norm_spec [delta; zeta] (llist_with_tail ptr [x]);
+  pure_star_interp (llist_with_tail_fragment ptr x []) (is_null (LL.next (L.last [x])) == true) m;
+  norm_spec [delta; zeta] (llist_with_tail_fragment ptr x []);
+  pure_star_interp (pts_to ptr.head full_perm x) (ptr.tail == ptr.head) m
+
+let intro_llist_cons_nil
+  (a: Type)
+  (ptr: t a)
+  (x: LL.cell a)
+: SteelT unit
+    (pts_to ptr.head full_perm x `star` pure (is_null (LL.next x) == true) `star` pure (ptr.tail == ptr.head))
+    (fun _ -> llist_with_tail ptr [x])
+=
+  change_slprop
+    (pts_to ptr.head full_perm x `star` pure (is_null (LL.next x) == true) `star` pure (ptr.tail == ptr.head))
+    (llist_with_tail ptr [x])
+    (fun m -> intro_llist_cons_nil' a ptr x m)
+
+let pts_to_not_null_intro
+  (#a:Type u#0)
+  (x:ref a)
+  (p:perm)
+  (v: Ghost.erased a)
+: SteelT unit (pts_to x p v) (fun _ -> pts_to x p v `star` pure (is_null x == false))
+=
+  change_slprop  (pts_to x p v) (pts_to x p v `star` pure (is_null x == false))
+  (fun m ->
+    pts_to_not_null x p v m;
+    pure_star_interp (pts_to x p v) (is_null x == false) m
+  )
+
+val intro_llist_cons_cons'
+  (a: Type)
+  (ptr: t a)
+  (ptr0 : t a)
+  (x: LL.cell a)
+  (q:  (list (LL.cell a)))
+  (m: mem)
+: Lemma
+  (requires (interp
+    (llist_with_tail ptr0 q `star` pts_to ptr.head full_perm x `star` pure (ptr0.head == LL.next x) `star` pure (ptr0.tail == ptr.tail) `star` pure (Cons? q == true))
+    m
+  ))
+  (ensures (interp
+    (llist_with_tail ptr (x :: q))
+  ) m)
+  (decreases q)
+
+let intro_llist_cons_cons'
+  a ptr ptr0 x q m
+=
+  (* destruct the hypothesis *)
+  pure_star_interp
+    (llist_with_tail ptr0 q `star` pts_to ptr.head full_perm x `star` pure (ptr0.head == LL.next x) `star` pure (ptr0.tail == ptr.tail))
+    (Cons? q == true)
+    m;
+  pure_star_interp
+    (llist_with_tail ptr0 q `star` pts_to ptr.head full_perm x `star` pure (ptr0.head == LL.next x))
+    (ptr0.tail == ptr.tail)
+    m;
+  pure_star_interp
+    (llist_with_tail ptr0 q `star` pts_to ptr.head full_perm x)
+    (ptr0.head == LL.next x)
+    m;
+  star_commutative
+    (llist_with_tail ptr0 q)
+    (pts_to ptr.head full_perm x);
+  llist_with_tail_cons ptr0 q;
+  star_associative
+    (pts_to ptr.head full_perm x)
+    (llist_with_tail_fragment ptr0 (L.hd q) (L.tl q))
+    (pure (is_null (LL.next (L.last q)) == true));
+  pure_star_interp
+    (pts_to ptr.head full_perm x `star` llist_with_tail_fragment ptr0 (L.hd q) (L.tl q))
+    (is_null (LL.next (L.last q)) == true)
+    m;
+  (* construct the conclusion *)
+  assert (ptr0 == ({ head = LL.next x; tail = ptr.tail }));
+  assert (L.last (x :: q) == L.last q);
+  llist_with_tail_fragment_cons ptr x q;
+  pure_star_interp
+    (llist_with_tail_fragment ptr x q)
+    (is_null (LL.next (L.last (x :: q))) == true)
+    m;
+  llist_with_tail_cons ptr (x :: q)
+
+let intro_llist_cons_cons
+  (a: Type)
+  (ptr: t a)
+  (ptr0 : t a)
+  (x: LL.cell a)
+  (q:  (list (LL.cell a)))
+: SteelT
+    unit
+    (llist_with_tail ptr0 q `star` pts_to ptr.head full_perm x `star` pure (ptr0.head == LL.next x) `star` pure (ptr0.tail == ptr.tail) `star` pure (Cons? q == true))
+    (fun _ -> llist_with_tail ptr (x :: q))
+=
+  change_slprop
+    (llist_with_tail ptr0 q `star` pts_to ptr.head full_perm x `star` pure (ptr0.head == LL.next x) `star` pure (ptr0.tail == ptr.tail) `star` pure (Cons? q == true))
+    (llist_with_tail ptr (x :: q))
+    (fun m -> intro_llist_cons_cons' a ptr ptr0 x q m)
+
+val push_cons_cons
+  (a: Type)
+  (ptr: t a)
+  (x: a)
+  (q: (list (LL.cell a)))
+: SteelT
+    (t a & (list (LL.cell a)))
+    (llist_with_tail ptr q `star` pure (Cons? q == true))
+    (fun z -> llist_with_tail (fst z) (snd z))
+
+#push-options "--ide_id_info_off"
+
+let push_cons_cons
+  a ptr0 e q
+=
+  let x = LL.mk_cell ptr0.head e in
+  let px = alloc x in
+  let ptr = {head = px ; tail = ptr0.tail} in
+  change_slprop
+    (pts_to px full_perm x)
+    (pts_to ptr.head full_perm x)
+    (fun _ -> ());
+  intro_pure (ptr0.head == LL.next x);
+  intro_pure (ptr0.tail == ptr.tail);
+  intro_llist_cons_cons a ptr ptr0 x q;
+  let z = (ptr, x :: q) in
+  z
 
